prove tctx_split_uniq_array; introduce JustLoc; fix proofs

theories/typing/array_idx.v
@@ -1,5 +1,6 @@
 From lrust.typing Require Export type.
-From lrust.typing Require Import programs array int shr_bor uniq_bor.
+From lrust.typing Require Import programs
+  array int shr_bor uniq_bor product product_split.
 Set Default Proof Using "Type".
 
 Implicit Type 𝔄: syn_type.
@@ -7,26 +8,26 @@ Implicit Type 𝔄: syn_type.
 Section lemmas.
   Context `{!typeG Σ}.
 
-  Lemma tctx_array_shr_idx {𝔄 𝔅l} (ty: _ 𝔄) n κ p (i: fin n) (T: _ 𝔅l) E L :
+  Lemma tctx_idx_shr_array {𝔄 𝔅l} (ty: _ 𝔄) n κ p (i: fin n) (T: _ 𝔅l) E L :
     tctx_incl E L (p ◁ &shr{κ} [ty; n] +:: T)
       (p +ₗ #(i * ty.(ty_size))%nat ◁ &shr{κ} ty +:: T)
       (λ post '(xl -:: bl), post (xl !!! i -:: bl))%type.
   Proof.
-    iIntros (??[vπ?]?) "_ _ _ _ $ [p T] Obs !>". iExists (_ -:: _).
+    iIntros (??[??]?) "_ _ _ _ $ [p T] Obs !>". iExists (_ -:: _).
     iFrame "Obs T". iDestruct "p" as ([[]|][|]Ev) "[⧖ ?]"=>//=. iExists _, _.
     iSplit; [by rewrite/= Ev|]. iFrame "⧖". by rewrite big_sepL_vlookup vfunsep_lookup.
   Qed.
 
-  Lemma tctx_extract_array_shr_idx {𝔄 𝔅l} (ty: _ 𝔄) n κ p (i: fin n) (T: _ 𝔅l) E L :
+  Lemma tctx_extract_idx_shr_array {𝔄 𝔅l} (ty: _ 𝔄) n κ p (i: fin n) (T: _ 𝔅l) E L :
     tctx_extract_elt E L (p +ₗ #(i * ty.(ty_size))%nat ◁ &shr{κ} ty)
       (p ◁ &shr{κ} [ty; n] +:: T) (p ◁ &shr{κ} [ty; n] +:: T)
       (λ post '(xl -:: bl), post (xl !!! i -:: xl -:: bl))%type.
   Proof.
     by eapply tctx_incl_eq; [eapply tctx_incl_trans;
-    [apply copy_tctx_incl, _|apply tctx_array_shr_idx]|].
+    [apply copy_tctx_incl, _|apply tctx_idx_shr_array]|].
   Qed.
 
-  Lemma type_array_shr_idx_instr {𝔄} (ty: _ 𝔄) n κ p q E L :
+  Lemma type_idx_shr_array_instr {𝔄} (ty: _ 𝔄) n κ p q E L :
     ⊢ typed_instr_ty E L +[p ◁ &shr{κ} [ty; n]; q ◁ int]
       (p +ₗ q * #ty.(ty_size))%E (&shr{κ} ty)
       (λ post '-[xl; z], ∃i: fin n, z = i ∧ post (xl !!! i))%type.
@@ -42,7 +43,7 @@ Section lemmas.
     by rewrite/= -Nat2Z.inj_mul big_sepL_vlookup vfunsep_lookup.
   Qed.
 
-  Lemma type_array_shr_idx {𝔄 𝔄l 𝔅l} (ty: _ 𝔄) n κ p q
+  Lemma type_idx_shr_array {𝔄 𝔄l 𝔅l} (ty: _ 𝔄) n κ p q
     (T: _ 𝔄l) (T': _ 𝔅l) tr pre x e E L C :
     Closed (x :b: []) e →
     tctx_extract_ctx E L +[p ◁ &shr{κ} [ty; n]; q ◁ int] T T' tr →
@@ -50,10 +51,37 @@ Section lemmas.
     typed_body E L C T (let: x := p +ₗ q * #ty.(ty_size) in e)
       (tr (λ '(xl -:: z -:: bl), ∃i: fin n, z = i ∧ pre (xl !!! i -:: bl)))%type.
   Proof.
-    iIntros. iApply type_let; [by apply type_array_shr_idx_instr|solve_typing| |done].
+    iIntros. iApply type_let; [by apply type_idx_shr_array_instr|solve_typing| |done].
     f_equal. fun_ext. by case=> [?[??]].
+  Qed.
+
+  Fixpoint hasty_uniq_idxs {𝔄} (p: path) (κ: lft) (ty: type 𝔄) (n: nat)
+    (i: nat) : tctx (replicate n (𝔄 * 𝔄)%ST) :=
+    match n with 0 => +[] | S m =>
+      p +ₗ #(i * ty.(ty_size))%nat ◁ &uniq{κ} ty +::
+      hasty_uniq_idxs p κ ty m (S i) end.
+
+  Lemma tctx_split_uniq_array {𝔄} (ty: _ 𝔄) n κ p E L :
+    lctx_lft_alive E L κ →
+    tctx_incl E L +[p ◁ &uniq{κ} [ty; n]] (hasty_uniq_idxs p κ ty n 0)
+      (λ post '-[(al, al')], post
+        (vec_to_plist (vzip al al': vec (𝔄 * 𝔄)%ST _))).
+  Proof.
+    move=> ?. move: p. elim: n. { move=> ?. eapply tctx_incl_eq;
+    [apply tctx_incl_leak_head|]=>/= ?[[v v'][]]. inv_vec v. by inv_vec v'. }
+    move=>/= n IH p. eapply tctx_incl_eq. { eapply tctx_incl_trans;
+    [eapply tctx_uniq_eqtype; by [apply array_succ_prod|apply _|]|].
+    eapply tctx_incl_trans. { eapply (tctx_incl_frame_r +[_]).
+    by eapply tctx_split_uniq_prod. } eapply (tctx_incl_app +[_] +[_]);
+    [apply tctx_to_shift_loc_0, _|]. eapply (tctx_incl_trans _ _ _ _ id); [apply IH|].
+    iIntros (???vπl?) "_ _ _ _ $ T Obs !>". iExists _. iFrame "Obs". clear.
+    move: 0=> k. iInduction n as [|] "IH" forall (p k); [done|]. case vπl=>/= ??.
+    iDestruct "T" as "[p T]". iSplitL "p"; [|by iApply "IH"].
+    rewrite tctx_elt_interp_hasty_path; [done|]=>/=. case (eval_path p)=>//.
+    (do 2 (case=>//))=> ?. by rewrite shift_loc_assoc -Nat2Z.inj_add. }
+    move=> ?[[v v'][]]. inv_vec v. by inv_vec v'.
   Qed.
 
 End lemmas.
 
-Global Hint Resolve tctx_extract_array_shr_idx | 5 : lrust_typing.
+Global Hint Resolve tctx_extract_idx_shr_array | 5 : lrust_typing.
